theories/iris/allocator/reprs.v
@@ -1,0 +1,294 @@
+From mathcomp Require Import ssreflect eqtype seq ssrbool.
+From iris.program_logic Require Import language.
+From iris.proofmode Require Import base tactics classes.
+From iris.base_logic Require Export gen_heap ghost_map proph_map na_invariants.
+From iris.base_logic.lib Require Export fancy_updates.
+From iris.bi Require Export weakestpre.
+From Wasm.iris.logrel Require Export iris_fundamental.
+From Wasm.iris.rules Require Export proofmode.
+From RWasm.iris.allocator Require Import allocator_common misc_relocate.
+
+Definition mem_block_at_pos_frac `{!wasmG Σ} (q: dfrac) (n: N) (l:bytes) k : iProp Σ :=
+  ([∗ list] i ↦ b ∈ l, n ↦[wm]{q} [ (N.of_nat (N.to_nat k+i)) ] b)%I.
+Locate "↦[wms][".
+
+Notation "n ↦[wms]{ q } [ i ] l" := (mem_block_at_pos_frac q n l i)                    
+                                      (at level 20, q at level 5, format "n ↦[wms]{ q } [ i ] l"): bi_scope.
+
+Section reprs.
+
+Context `{!wasmG Σ}. 
+
+Inductive state_flag :=
+| Used
+| Free
+| Final.
+
+Inductive block : Type :=
+| UsedBlk
+    (blk_used_size: N)
+    (blk_leftover_size: N)
+    (*(blk_padding: iProp Σ)*)
+| FreeBlk
+    (blk_size: N).
+
+Inductive final_block : Type :=
+| FinalBlk
+    (blk_size: N).
+
+Definition blocks : Type :=
+  list block * final_block.
+
+(* beware:
+    The i32 type is a record {intval: Z; proof: -1 < z < 2^32}.
+    This means that nat_repr is not a functional relation
+    (unless you assume propositional extensionality).
+*)
+Definition nat_repr (n: nat) (n32: i32) : Prop :=
+  (-1 < Z.of_nat n < Wasm_int.Int32.modulus)%Z /\
+  n = Wasm_int.nat_of_uint i32m n32.
+
+(* beware:
+    The i32 type is a record {intval: Z; proof: -1 < z < 2^32}.
+    This means that N_repr is not a functional relation
+    (unless you assume propositional extensionality).
+*)
+Definition N_repr (n: N) (n32: i32) : Prop :=
+  (-1 < Z.of_N n < Wasm_int.Int32.modulus)%Z /\
+  n = Wasm_int.N_of_uint i32m n32.
+
+Lemma N_repr_uint:
+  forall n n32,
+    N_repr n n32 ->
+    n = Wasm_int.N_of_uint i32m n32.
+Proof.
+  unfold N_repr.
+  tauto.
+Qed.
+
+Lemma N_repr_i32repr: 
+  forall (n: N) (z: Z),
+    (-1 < Z.of_N n < Wasm_int.Int32.modulus)%Z ->
+    z = Z.of_N n ->
+    N_repr n (Wasm_int.Int32.repr z).
+Proof.
+  intros.
+  unfold Wasm_int.Int32.repr, N_repr, Wasm_int.N_of_uint; cbn.
+  split.
+  - lia.
+  - rewrite Wasm_int.Int32.Z_mod_modulus_id.
+    + subst. by rewrite N2Z.id.
+    + lia.
+Qed.
+
+Definition block_flag blk :=
+  match blk with
+  | UsedBlk _ _ => Used
+  | FreeBlk _ => Free
+  end.
+
+Definition final_block_flag blk :=
+  match blk with
+  | FinalBlk _ => Final
+  end.
+
+Definition block_size blk : N :=
+  match blk with
+  | UsedBlk sz_u sz_l => sz_u + sz_l
+  | FreeBlk sz => sz
+  end.
+
+Definition state_to_N (flag : state_flag) : N :=
+  match flag with
+  | Used => BLK_USED
+  | Free => BLK_FREE
+  | Final => BLK_FINAL
+  end.
+
+Definition state_frac flag : Qp :=
+  match flag with
+  | Used => 1/2
+  | _ => 1
+  end.
+
+Lemma mem_block_at_frac_one n i l :
+  n ↦[wms]{DfracOwn 1}[i] l ⊢ n ↦[wms][i] l.
+Proof.
+  iIntros.
+  iFrame.
+Qed.
+    
+
+Lemma mem_block_at_frac_combine n p q i l l' :
+  n ↦[wms]{p}[i] l ∗ n ↦[wms]{q}[i] l' ⊢ n ↦[wms]{p ⋅ q}[i] l ∗ ⌜l = l'⌝.
+Proof.
+Admitted.
+
+Lemma mem_block_at_frac_split n p q i l :
+  n ↦[wms]{p ⋅ q}[i] l ⊢
+  n ↦[wms]{p}[i] l ∗ n ↦[wms]{q}[i] l.
+Proof.
+Admitted.
+
+Lemma mem_block_at_frac_halve n i l :
+  n ↦[wms][i] l ⊢
+  n ↦[wms]{DfracOwn (1/2)}[i] l ∗ n ↦[wms]{DfracOwn (1/2)}[i] l.
+Proof.
+  iIntros "H".
+  iApply mem_block_at_frac_split.
+  rewrite dfrac_op_own.
+  rewrite Qp.half_half.
+  iFrame.
+Qed.
+
+Definition own_vec (memidx: N) (base_addr: N) (sz: N) : iProp Σ :=
+  ∃ bs: bytes, ⌜N.of_nat (length bs) = sz⌝ ∗ memidx ↦[wms][base_addr] bs.
+
+Definition own_half_vec (memidx: N) (base_addr: N) (sz: N) : iProp Σ :=
+  ∃ bs: bytes, ⌜N.of_nat (length bs) = sz⌝ ∗ memidx ↦[wms]{DfracOwn (1/2)}[base_addr] bs.
+
+Lemma own_half_vec_split memidx base_addr sz:
+  own_half_vec memidx base_addr sz ∗ own_half_vec memidx base_addr sz ⊣⊢ own_vec memidx base_addr sz.
+Proof.
+  iSplit.
+  - iIntros "[[%b [%len H]] [%b' [%len' H']]]".
+    iPoseProof (mem_block_at_frac_combine with "[$]") as "[Hcomb %Hbeq]".
+    subst b'.
+    rewrite dfrac_op_own.
+    rewrite Qp.half_half.
+    iExists b.
+    by iFrame.
+  - iIntros "(%b & %bsz & H)".
+    iPoseProof (mem_block_at_frac_halve with "[$]") as "[Hp Hq]".
+    by iFrame.
+Qed.
+
+Eval vm_compute in bits (VAL_int32 (Wasm_int.Int32.repr (Z.of_N (state_to_N Used)))).
+Definition alloc_tok (memidx: N) (data_addr: N) : iProp Σ :=
+  ∃ st,
+    ⌜N_repr (state_to_N Used) st⌝ ∗
+     memidx ↦[wms]{DfracOwn (1/2)}[data_addr - data_off + state_off] bits (VAL_int32 st).
+
+Definition state_repr (memidx: N) (flag: state_flag) (base_addr: N) : iProp Σ :=
+  ∃ st,
+    ⌜N_repr (state_to_N flag) st⌝ ∗
+    memidx ↦[wms]{DfracOwn (state_frac flag)}[base_addr + state_off] bits (VAL_int32 st).
+
+Definition size_repr (memidx: N) (sz: N) (base_addr: N) : iProp Σ :=
+  ∃ sz32,
+    ⌜N_repr sz sz32 ⌝ ∗
+    memidx ↦[wms][base_addr + size_off] bits (VAL_int32 sz32).
+
+Definition next_repr (memidx: N) (next: N) (base_addr: N) : iProp Σ :=
+  ∃ next32,
+    ⌜N_repr next next32 ⌝ ∗
+  memidx ↦[wms][base_addr + next_off] bits (VAL_int32 next32).
+
+Definition data_repr memidx blk base_addr :=
+  match blk with
+  | UsedBlk blk_used_size blk_leftover_size =>
+      own_vec memidx (base_addr + data_off + blk_used_size) blk_leftover_size
+  | FreeBlk blk_size =>
+      own_vec memidx (base_addr + data_off) blk_size
+  end.
+
+Definition block_inbounds (memidx: N) (blk_size: N) (base_addr: N) : iProp Σ :=
+  ⌜(Z.of_N (base_addr + blk_hdr_sz + blk_size) < Wasm_int.Int32.modulus)%Z⌝.
+
+Definition block_repr (memidx: N) (blk: block) (base_addr next_addr: N) : iProp Σ :=
+  block_inbounds memidx (block_size blk) base_addr ∗
+  state_repr memidx (block_flag blk) base_addr ∗
+  size_repr memidx (block_size blk) base_addr ∗
+  next_repr memidx next_addr base_addr ∗
+  data_repr memidx blk base_addr.
+
+(* 
+EXTERNAL SPEC
+blks "allocator state"
+1. Allocator invariant   freelist_repr blks 0
+2. Allocation token      Allocated(blks, l, sz) <---> In (UsedBlk sz) blks
+
+
+                                    { AInv(st) } malloc(sz) { v. exists st'. v |-> bs * |bs| = sz * tok(st', v) * AInv(st') }
+{ AInv(st) * v |-> bs * |bs| = sz * tok(st, v) } free(v)    { (). exists st'. AInv(st') }
+own_block (N.of_nat memidx) ret_addr reqd_sz ∗
+*)
+
+Fixpoint blocks_repr (memidx: N) (blks: list block) (base_addr: N) (out_addr: N) : iProp Σ :=
+  match blks with
+  | blk :: blks =>
+      ∀ next_addr,
+        block_repr memidx blk base_addr next_addr ∗
+        blocks_repr memidx blks next_addr out_addr
+  | [] =>
+      ⌜base_addr = out_addr⌝
+  end.
+
+Definition final_block_repr (memidx: N) (blk: final_block) (base_addr: N) : iProp Σ :=
+  match blk with
+  | FinalBlk blk_size =>
+      block_inbounds memidx blk_size base_addr ∧
+      state_repr memidx Final base_addr ∗
+      size_repr memidx blk_size base_addr ∗
+      next_repr memidx 0%N base_addr ∗
+      own_vec memidx (base_addr + data_off) blk_size
+  end.
+
+Definition final_block_sz (blk: final_block) : N :=
+  match blk with
+  | FinalBlk sz => sz
+  end.
+
+Lemma final_block_inbounds (memidx: N) (blk: final_block) (base_addr: N) :
+  ⊢ final_block_repr memidx blk base_addr -∗
+    ⌜(Z.of_N (base_addr + blk_hdr_sz + final_block_sz blk) < Wasm_int.Int32.modulus)%Z⌝ ∗
+    final_block_repr memidx blk base_addr.
+Proof.
+  iIntros "H".
+  destruct blk.
+  iDestruct "H" as "(%Hinbounds & H')".
+  iFrame; auto.
+Qed.
+
+Definition freelist_repr (memidx: N) (blks: list block * final_block) (base_addr: N) : iProp Σ :=
+  let '(blks, final) := blks in
+  ∀ next_addr,
+    blocks_repr memidx blks base_addr next_addr ∗
+    final_block_repr memidx final next_addr.
+
+Lemma own_vec_split memidx ℓ sz1 sz2 :
+  own_vec memidx ℓ (sz1 + sz2) ⊣⊢ own_vec memidx ℓ sz1 ∗ own_vec memidx (ℓ + sz1) sz2.
+Proof.
+  unfold own_vec.
+  iSplit.
+  - iIntros "(%bs & %Hlen & Hbs)".
+    pose proof (take_drop (N.to_nat sz1) bs) as Hsplit.
+    rewrite <- Hsplit.
+    rewrite wms_app; [|eauto; lia].
+    iDestruct "Hbs" as "(Hbs1 & Hbs2)".
+    iSplitL "Hbs1".
+    + iExists _; iFrame.
+      iPureIntro.
+      rewrite length_take_le; lia.
+    + rewrite length_take_le; [|lia].
+      rewrite N2Nat.id.
+      iExists _; iFrame.
+      iPureIntro.
+      rewrite length_drop.
+      lia.
+  - iIntros "((%bs1 & (%Hlen1 & Hbs1)) & (%bs2 & (%Hlen2 & Hbs2)))".
+    iExists (bs1 ++ bs2).
+    erewrite (wms_app _ _ _ (sz1:=sz1)); [| lia].
+    iFrame.
+    iPureIntro.
+    rewrite length_app.
+    lia.
+Qed.
+
+Lemma serialise_i32_inj:
+  forall i k,
+    serialise_i32 i = serialise_i32 k ->
+    i = k.
+Admitted.
+
+End reprs.
